coq/theories/utils/Llist.v
@@ -8,3 +8,9 @@ Definition ltail {A : Type} (l : llist A) : llist A :=
   | Lnil => Lnil
   | Lcons _ tl => tl
   end.
+
+Fixpoint llist_of_list {A: Type} (l: list A): llist A :=
+  match l with
+  | nil => Lnil
+  | cons x xs => Lcons x (llist_of_list xs)
+  end.
